STDIO: new definition and main_thm

basis/fsioProgConstantsScript.sml
@@ -55,8 +55,7 @@ val FILENAME_def = Define `
 (* abstracts away the lazy list and ensure that standard streams are opened on
 * their respective standard fds at the right position *)
 val STDIO_def = Define`
- STDIO fs = SEP_EXISTS k. 
-   IOFS (fs with numchars := THE (LDROP k fs.numchars)) *
+ STDIO fs = (SEP_EXISTS ll. IOFS (fs with numchars := ll)) *
    &(? inp out err. 
         (ALOOKUP fs.infds 0 = SOME (strlit "stdin", inp)) ∧
         (ALOOKUP fs.infds 1 = SOME (strlit "stdout", LENGTH out)) ∧
@@ -134,18 +133,42 @@ val EndOfFile_UNICITY = Q.store_thm("EndOfFile_UNICITY[xlet_auto_match]",
 `!v1 v2. EndOfFile_exn v1 ==> (EndOfFile_exn v2 <=> v2 = v1)`,
   fs[EndOfFile_exn_def]);
 
-
 val UNIQUE_STDIO = Q.store_thm("UNIQUE_STDIO",
 `!s. VALID_HEAP s ==> !fs1 fs2 H1 H2. (STDIO fs1 * H1) s /\
                                       (STDIO fs2 * H2) s ==> 
-     ?k1 k2. (THE(LDROP k1 fs1.numchars) = THE(LDROP k2 fs2.numchars)) /\
-             (IOFS (fs1 with numchars := THE(LDROP k1 fs1.numchars)) * H1) s`,
-  rw[STDIO_def,SEP_CLAUSES,SEP_EXISTS_THM] >>
-  qexists_tac`k` >> qexists_tac`k'` >> rw[] >>
-  fs[STAR_COMM,STAR_ASSOC,cond_STAR] >>
+              (fs1.infds = fs2.infds /\ fs1.files = fs2.files)`,
+  rw[STDIO_def,SEP_CLAUSES,SEP_EXISTS_THM,STAR_COMM,STAR_ASSOC,cond_STAR] >>
   fs[Once STAR_COMM] >>
   imp_res_tac UNIQUE_IOFS >>
   cases_on`fs1` >> cases_on`fs2` >> fs[IO_fs_numchars_fupd]);
+
+(* weak injection theorem *)
+val STDIO_HPROP_INJ = Q.store_thm("STDIO_HPROP_INJ[hprop_inj]",
+`HPROP_INJ (STDIO fs1) (STDIO fs2) 
+           (fs1.infds = fs2.infds /\ fs1.files = fs2.files)`,
+  rw[HPROP_INJ_def, GSYM STAR_ASSOC, SEP_CLAUSES, SEP_EXISTS_THM,
+     HCOND_EXTRACT] >>
+  EQ_TAC >> rpt DISCH_TAC
+  >-(mp_tac UNIQUE_STDIO >> disch_then drule >>
+     strip_tac >> 
+     first_x_assum (qspecl_then [`fs1`, `fs2`] mp_tac) >>
+     rpt (disch_then drule) >> fs[cond_def] >> rw[] >>
+     fs[STDIO_def,STAR_def,SEP_EXISTS,cond_def] >>
+     qmatch_assum_rename_tac`IOFS (fs2 with numchars := ll) u1` >>
+     qmatch_assum_rename_tac`SPLIT u0 (u1, _)` >>
+     qmatch_assum_rename_tac`SPLIT s (u0, v0)` >>
+     qexists_tac`u0` >> qexists_tac`v0` >> fs[] >>
+     qexists_tac`u1` >> fs[] >> qexists_tac`ll` >> fs[] >>
+     cases_on`fs1` >> cases_on`fs2` >> fs[IO_fs_numchars_fupd]
+     ) >>
+  fs[STDIO_def,STAR_def,SEP_EXISTS,cond_def] >>
+  qmatch_assum_rename_tac`IOFS (fs1 with numchars := ll) u1` >>
+  qmatch_assum_rename_tac`SPLIT u0 (u1, _)` >>
+  qmatch_assum_rename_tac`SPLIT s (u0, v0)` >>
+  qexists_tac`u0` >> qexists_tac`v0` >> fs[] >>
+  qexists_tac`u1` >> fs[] >> qexists_tac`ll` >> fs[] >>
+  cases_on`fs1` >> cases_on`fs2` >> fs[IO_fs_numchars_fupd] >>
+  metis_tac[]);
 
 val _ = export_theory();
 
